Diff/LanguageModel.v
@@ -129,3 +129,39 @@ Proof.
   apply Hsuper.
   now apply (rsat1 C).
 Qed. 
+
+
+Definition sat2 {L : Language}
+                {trace_set : Set}
+                (S : Semantics L trace_set)
+                (W1 W2 : prg L) (R : trace_set * trace_set -> Prop) : Prop :=
+  forall t1 t2, sem S W1 t1 -> sem S W2 t2 -> R (t1, t2).
+
+Definition rsat2 {L : Language}
+                 {trace_set : Set}
+                 (S : Semantics L trace_set)
+                 (P1 P2 : par L) (R : trace_set * trace_set -> Prop) : Prop :=
+  forall C t1 t2, sem S (plug L P1 C) t1 -> sem S (plug L P2 C) t2 -> R (t1, t2).
+
+Lemma sat2_upper_closed  {L : Language}
+                         {trace_set : Set}
+                         (S : Semantics L trace_set)
+                         (W1 W2 : prg L ) (R1 R2 : trace_set * trace_set -> Prop) :
+  sat2 S W1 W2 R1 -> R1 ⊆ R2 -> sat2 S W1 W2 R2.
+Proof.
+  intros Hsat1 Hsuper t1 t2 Hsem1 Hsem2.
+  apply Hsuper.
+  now apply (Hsat1 t1).
+Qed.
+
+Lemma rsat2_upper_closed {L : Language}
+                         {trace_set : Set}
+                         (S : Semantics L trace_set)
+                         (P1 P2 : par L ) (R1 R2 : trace_set * trace_set -> Prop) :
+  rsat2 S P1 P2 R1 -> R1 ⊆ R2 -> rsat2 S P1 P2 R2.
+Proof.
+  intros Hsat1 Hsuper C t1 t2 Hsem1 Hsem2.
+  apply Hsuper.
+  now apply (Hsat1 C t1).
+Qed.
+
