Diff/Robust2relTraceProperty.v
@@ -1,0 +1,115 @@
+From mathcomp Require Import all_ssreflect.
+
+Set Implicit Arguments.
+Unset Printing Implicit Defensive.
+
+Require Import ClassicalExtras.
+Require Import MyNotation.
+Require Import Setoid.
+Require Import FunctionalExtensionality.
+
+Require Import Galois.
+Require Import LanguageModel.
+Require Import TraceModel.
+Require Import Properties.
+Require Import ChainModel.
+
+Hypothesis prop_extensionality : forall A B : Prop, (A <-> B) -> A = B.
+
+Section Robust2relPreservation.
+
+  Variable Source Target: Language.
+  Variable compilation_chain : CompilationChain Source Target.
+
+  (*CA: we don't need a particular structure of traces to define preservation
+        e.g. traces = values or our defn of traces both make sense
+   *)
+  Variable trace__S trace__T : Set.
+
+  Local Definition prop__S := prop trace__S.
+  Local Definition prop__T := prop trace__T.
+
+  Variable Source_Semantics : Semantics Source trace__S.
+  Variable Target_Semantics : Semantics Target trace__T.
+
+  Local Definition sem__S := sem Source_Semantics.
+  Local Definition sem__T := sem Target_Semantics.
+  Local Definition par__S := par Source.
+  Local Definition par__T := par Target.
+  Local Definition ctx__S := ctx Source.
+  Local Definition ctx__T := ctx Target. 
+  Local Definition rsat__S := rsat2 Source_Semantics.
+  Local Definition rsat__T := rsat2 Target_Semantics.
+  
+  Local Definition cmp := compile_par Source Target compilation_chain.
+
+  Local Notation "P ↓" := (cmp P) (at level 50).
+ (* CA: don't understand why this does not work 
+
+   Local Notation " C [ P ] " := (plug _  P C) (at level 50).
+  *)
+  Local Definition plug__S:= plug Source.
+  Local Definition plug__T := plug Target.
+  
+  Variable σ : (trace__T * trace__T -> Prop) -> (trace__S * trace__S -> Prop).
+  Variable τ : (trace__S * trace__S -> Prop) -> (trace__T * trace__T -> Prop).
+
+  Definition σR2P (P1 P2 : par__S) (T : trace__T * trace__T -> Prop) :=
+    rsat__S P1 P2 (σ T) -> rsat__T (P1 ↓) (P2 ↓) T.   
+
+  Definition σR2TP := forall P1 P2 T, σR2P P1 P2 T.
+
+  (* Lemma contra_σRP (P : par__S) (π__T : prop__T) : *)
+  (*   (σRP P π__T) <->  ((exists C__T t, sem__T ( plug__T (P↓) C__T) t /\ ~ (π__T t)) -> *)
+  (*                  (exists C__S s, sem__S ( plug__S  P C__S) s /\ ~ (σ π__T) s)). *)
+  (* Proof. *)
+  (*   rewrite /σRP. by rewrite [_ -> _] contra !neg_rsat. *)
+  (* Qed. *)
+
+  (* Lemma contra_σRTP : *)
+  (*   σRTP <-> (forall P π__T, (exists C__T t, sem__T (plug__T (P ↓) C__T) t /\ ~ (π__T t)) -> *)
+  (*                    (exists C__S s, sem__S (plug__S P C__S) s /\ ~ (σ π__T) s)). *)
+  (* Proof. *)
+  (*   rewrite /σRTP. *)
+  (*   split => H P π__T; by move/contra_σRP: (H P π__T). *)
+  (* Qed. *)
+
+  Definition τR2P (P1 P2 : par__S) (S : trace__S * trace__S -> Prop) :=
+    rsat__S P1 P2 S -> rsat__T (P1 ↓) (P2 ↓) (τ S).
+
+  Definition τR2TP := forall P1 P2 S, τR2P P1 P2 S.
+
+  (* Lemma contra_τRP (P : par__S) (π__S : prop__S) : *)
+  (*   (τRP P π__S) <-> ((exists C__T t, sem__T ( plug__T (P↓) C__T) t /\ ~ (τ π__S) t) -> *)
+  (*                (exists C__S s, sem__S (plug__S P C__S) s /\ ~ π__S s)). *)
+  (* Proof. *)
+  (*   rewrite /τRP. by rewrite [_ -> _] contra !neg_rsat. *)
+  (* Qed. *)
+
+  (* Lemma contra_τRTP : *)
+  (*   τRTP <-> (forall P π__S, ((exists C__T t, sem__T ( plug__T (P↓) C__T) t /\ ~ (τ π__S) t) -> *)
+  (*                    (exists C__S s, sem__S (plug__S P C__S) s /\ ~ π__S s))). *)
+  (* Proof. *)
+  (*   rewrite /τRTP. *)
+  (*   split => H P π__S; by move/contra_τRP: (H P π__S). *)
+  (* Qed. *)
+
+  Theorem G_σRTP_iff_τRTP :
+    (Galois_fst τ σ) -> (Galois_snd τ σ) -> (σR2TP <-> τR2TP).
+  Proof.
+    move => G1 G2. split.
+    - move => Hσ P1 P2 S Hrsat_src. apply: (Hσ P1 P2 (τ S)).
+      apply: rsat2_upper_closed. exact Hrsat_src. by apply: G1.
+    - move => Hτ P1 P2 T Hrrsat_tgt.
+      have H : rsat__T (P1 ↓) (P2 ↓) (τ (σ T)) by apply: Hτ.
+      apply: rsat2_upper_closed. exact H. by apply: G2.
+  Qed.
+
+  Corollary Adj_σRTP_iff_τRTP :
+    Adjunction_law τ σ -> (σR2TP <-> τR2TP).
+  Proof.
+    rewrite Galois_equiv. move => [ms [mt [G1 G2]]].
+      by apply: G_σRTP_iff_τRTP.
+  Qed.
+
+End Robust2relPreservation.
